Prefix: : <http://www.semanticweb.org/singh/ontologies/2020/2/CW2#>
Prefix: dc: <http://purl.org/dc/elements/1.1/>
Prefix: owl: <http://www.w3.org/2002/07/owl#>
Prefix: rdf: <http://www.w3.org/1999/02/22-rdf-syntax-ns#>
Prefix: rdfs: <http://www.w3.org/2000/01/rdf-schema#>
Prefix: xml: <http://www.w3.org/XML/1998/namespace>
Prefix: xsd: <http://www.w3.org/2001/XMLSchema#>



Ontology: <http://www.semanticweb.org/singh/ontologies/2020/2/CW2>

Import: <http://www.movieontology.org/2009/11/09/movieontology.owl>

AnnotationProperty: <http://www.w3.org/2004/02/skos/core#broader>

    
AnnotationProperty: <http://www.w3.org/2004/02/skos/core#narrower>

    
AnnotationProperty: owl:sameAs

    
AnnotationProperty: rdfs:comment

    
AnnotationProperty: rdfs:label

    
Datatype: rdf:PlainLiteral

    
Datatype: xsd:int

    
Datatype: xsd:string

    
ObjectProperty: hasActor

    Annotations: 
        rdfs:comment "Movie which has a male actor in it",
        rdfs:label <http://www.semanticweb.org/singh/ontologies/2020/2/CW2#hasActor>,
        owl:sameAs <http://www.movieontology.org/2009/10/01/movieontology.owl#hasMaleActor>
    
    Domain: 
        Movie
    
    InverseOf: 
        isActorIn
    
    
ObjectProperty: hasActress

    Annotations: 
        rdfs:comment "Movie has a female actress in it",
        rdfs:label <http://www.semanticweb.org/singh/ontologies/2020/2/CW2#hasActress>,
        owl:sameAs <http://www.movieontology.org/2009/10/01/movieontology.owl#hasActress>
    
    Domain: 
        Movie
    
    InverseOf: 
        isActressIn
    
    
ObjectProperty: hasDirector

    Annotations: 
        rdfs:comment "Movie has a Director who directs it",
        rdfs:label <http://www.semanticweb.org/singh/ontologies/2020/2/CW2#hasDirector>,
        owl:sameAs <http://www.movieontology.org/2009/10/01/movieontology.owl#hasDirector>
    
    Domain: 
        Movie
    
    Range: 
        Director
    
    InverseOf: 
        isDirectorOf
    
    
ObjectProperty: hasEditor

    Annotations: 
        rdfs:comment "Movie has an Editor that edits it",
        rdfs:label <http://www.semanticweb.org/singh/ontologies/2020/2/CW2#hasEditor>,
        owl:sameAs <http://www.movieontology.org/2009/10/01/movieontology.owl#hasEditor>
    
    Characteristics: 
        Asymmetric
    
    Domain: 
        Movie
    
    Range: 
        Editor
    
    InverseOf: 
        isEditorOf
    
    
ObjectProperty: hasGenre

    SubPropertyOf: 
        owl:topObjectProperty
    
    Domain: 
        <http://www.movieontology.org/2009/11/09/Movie>
    
    Range: 
        Genre
    
    InverseOf: 
        isGenreOf
    
    
ObjectProperty: hasProducer

    Annotations: 
        rdfs:comment "Movie has a Producer that produces it",
        rdfs:label <http://www.semanticweb.org/singh/ontologies/2020/2/CW2#hasProducer>,
        owl:sameAs <http://www.movieontology.org/2009/10/01/movieontology.owl#hasProducer>
    
    Characteristics: 
        Asymmetric
    
    Domain: 
        Movie
    
    Range: 
        Producer
    
    InverseOf: 
        isProducerOf
    
    
ObjectProperty: hasRated

    Characteristics: 
        Asymmetric
    
    Domain: 
        User,
        hasRated some Rating
    
    Range: 
        Movie
    
    InverseOf: 
        isRatedBy
    
    
ObjectProperty: hasReviewer

    Annotations: 
        rdfs:comment "Movie has a Reviewer who reviews it",
        rdfs:label <http://www.semanticweb.org/singh/ontologies/2020/2/CW2#hasReviewer>
    
    Characteristics: 
        Asymmetric
    
    Domain: 
        Movie
    
    Range: 
        Reviewer
    
    InverseOf: 
        isReviewerOf
    
    
ObjectProperty: hasWriter

    Annotations: 
        rdfs:comment "Movie has a writer who writes its script",
        rdfs:label <http://www.semanticweb.org/singh/ontologies/2020/2/CW2#hasWriter>
    
    Domain: 
        Movie
    
    Range: 
        Writer
    
    InverseOf: 
        isWriterOf
    
    
ObjectProperty: isActorIn

    Annotations: 
        rdfs:comment "A male actor who acts in a movie",
        rdfs:label <http://www.semanticweb.org/singh/ontologies/2020/2/CW2#isActorIn>,
        owl:sameAs <http://www.movieontology.org/2009/11/09/movieontology.owl#isMaleActorIn>
    
    DisjointWith: 
        isActressIn
    
    Domain: 
        Actor
    
    Range: 
        Movie
    
    InverseOf: 
        hasActor
    
    
ObjectProperty: isActressIn

    Annotations: 
        rdfs:comment "A femal actor who acts in a movie",
        rdfs:label <http://www.semanticweb.org/singh/ontologies/2020/2/CW2#isActressIn>,
        owl:sameAs <http://www.movieontology.org/2009/10/01/movieontology.owl#isActressIn>
    
    DisjointWith: 
        isActorIn
    
    Domain: 
        Actor
    
    Range: 
        Movie
    
    InverseOf: 
        hasActress
    
    
ObjectProperty: isDirectorOf

    Annotations: 
        rdfs:comment "A Director who directs a movie",
        rdfs:label <http://www.semanticweb.org/singh/ontologies/2020/2/CW2#isDirectorOf>,
        owl:sameAs <http://www.movieontology.org/2009/10/01/movieontology.owl#isDirectorOf>,
        <http://www.w3.org/2004/02/skos/core#broader> <http://www.ime.usp.br/~renata/FOAF-modifiedmaker>
    
    Domain: 
        Director
    
    Range: 
        Movie
    
    InverseOf: 
        hasDirector
    
    
ObjectProperty: isEditorOf

    Annotations: 
        rdfs:comment "An Editor who edits a movie",
        rdfs:label <http://www.semanticweb.org/singh/ontologies/2020/2/CW2#isEditorOf>,
        owl:sameAs <http://www.movieontology.org/2009/10/01/movieontology.owl#isEditorIn>
    
    Domain: 
        Editor
    
    Range: 
        Movie
    
    InverseOf: 
        hasEditor
    
    
ObjectProperty: isGenreOf

    SubPropertyOf: 
        owl:topObjectProperty
    
    Domain: 
        Genre
    
    Range: 
        <http://www.movieontology.org/2009/11/09/Movie>
    
    InverseOf: 
        hasGenre
    
    
ObjectProperty: isProducerOf

    Annotations: 
        rdfs:comment "A Producer who produces a movie",
        rdfs:label <http://www.semanticweb.org/singh/ontologies/2020/2/CW2#isProducerOf>,
        owl:sameAs <http://www.movieontology.org/2009/10/01/movieontology.owl#isProducedBy>,
        owl:sameAs <http://www.movieontology.org/2009/10/01/movieontology.owl#produced>
    
    Domain: 
        Producer
    
    Range: 
        Movie
    
    InverseOf: 
        hasProducer
    
    
ObjectProperty: isRatedBy

    Domain: 
        Movie
    
    Range: 
        User
    
    InverseOf: 
        hasRated
    
    
ObjectProperty: isReviewerOf

    Annotations: 
        rdfs:comment "A Reviewer who reviews a movie",
        rdfs:label <http://www.semanticweb.org/singh/ontologies/2020/2/CW2#isReviewerOf>
    
    Domain: 
        Reviewer
    
    Range: 
        Movie
    
    InverseOf: 
        hasReviewer
    
    
ObjectProperty: isWriterOf

    Annotations: 
        rdfs:comment "A Writer who writes the script of a movie",
        rdfs:label <http://www.semanticweb.org/singh/ontologies/2020/2/CW2#isWriterOf>
    
    Domain: 
        Writer
    
    Range: 
        Movie
    
    InverseOf: 
        hasWriter
    
    
ObjectProperty: owl:topObjectProperty

    
DataProperty: ID

    Domain: 
        User
    
    Range: 
        xsd:int
    
    
DataProperty: firstName

    Domain: 
        Person
    
    Range: 
        xsd:string
    
    
DataProperty: lastName

    Domain: 
        Person
    
    Range: 
        xsd:string
    
    
DataProperty: releaseYear

    Annotations: 
        rdfs:comment "releaseYear is sameAs releaseDate, conceptually they represent same idea",
        owl:sameAs <http://www.movieontology.org/2009/10/01/movieontology.owl#releasedate>
    
    Domain: 
        Movie
    
    Range: 
        xsd:int
    
    
DataProperty: runtime

    Annotations: 
        rdfs:comment "runtime is sameAs runtime, conceptually they represent same idea and act on same domain and range",
        owl:sameAs <http://www.movieontology.org/2009/10/01/movieontology.owl#runtime>
    
    Domain: 
        Movie
    
    Range: 
        xsd:int
    
    
Class: <http://www.movieontology.org/2009/11/09/Movie>

    
Class: Actor

    Annotations: 
        rdfs:comment "A person who acts in a movie",
        rdfs:label <http://www.semanticweb.org/singh/ontologies/2020/2/CW2#Actor>,
        owl:sameAs <http://dbpedia.org/ontology/Actor>,
        <http://www.w3.org/2004/02/skos/core#broader> <http://www.ime.usp.br/~renata/FOAF-modifiedPerson>
    
    EquivalentTo: 
        Person
         and (isActorIn some Movie)
    
    SubClassOf: 
        Person
    
    
Class: Director

    Annotations: 
        rdfs:comment "A person who directs a movie",
        rdfs:label "Director",
        owl:sameAs <http://dbpedia.org/page/Film_Director>,
        <http://www.w3.org/2004/02/skos/core#broader> <http://www.ime.usp.br/~renata/FOAF-modifiedPerson>
    
    EquivalentTo: 
        Person
         and (isDirectorOf some Movie)
    
    SubClassOf: 
        Person
    
    
Class: Editor

    Annotations: 
        rdfs:comment "A person who edits a movie",
        rdfs:label "Editor",
        owl:sameAs <http://www.movieontology.org/2009/10/01/movieontology.owl#Editor>,
        <http://www.w3.org/2004/02/skos/core#broader> <http://www.ime.usp.br/~renata/FOAF-modifiedPerson>
    
    EquivalentTo: 
        Person
         and (isEditorOf some Movie)
    
    SubClassOf: 
        Person
    
    
Class: FeatureLengthFilm

    Annotations: 
        rdfs:comment "Movie from target ontology is broader than FeatureLengthFilm as FeatureLengthFilm is a Movie but also has a runtime greater than 40 minutes",
        rdfs:label <http://www.semanticweb.org/singh/ontologies/2020/2/CW2#FeatureLengthFilm>,
        <http://www.w3.org/2004/02/skos/core#broader> <http://www.movieontology.org/2009/11/09/Movie>
    
    EquivalentTo: 
        Movie
         and (runtime some xsd:int[> "40"^^xsd:int])
    
    SubClassOf: 
        Movie
    
    DisjointWith: 
        ShortFilm
    
    
Class: Genre

    Annotations: 
        rdfs:comment "This class defines the category genres of the movies or films. Not all films have a genre and films can have multiple genres.",
        rdfs:label <http://www.semanticweb.org/singh/ontologies/2020/2/CW2#Genre>,
        owl:sameAs <http://www.movieontology.org/2009/10/01/movieontology.owl#Genre>
    
    
Class: Movie

    Annotations: 
        owl:sameAs <http://www.movieontology.org/2009/11/09/Movie>
    
    
Class: Person

    
Class: Producer

    Annotations: 
        rdfs:comment "A person who produces a movie",
        rdfs:label "Producer",
        owl:sameAs <http://www.movieontology.org/2009/10/01/movieontology.owl#Producer>,
        <http://www.w3.org/2004/02/skos/core#broader> <http://www.ime.usp.br/~renata/FOAF-modifiedPerson>
    
    EquivalentTo: 
        Person
         and (isProducerOf some Movie)
    
    SubClassOf: 
        Person
    
    
Class: Rating

    Annotations: 
        rdfs:comment "Is a number value given to a movie based on a personal experience of viewing the movie",
        rdfs:label <http://www.semanticweb.org/singh/ontologies/2020/2/CW2#Rating>
    
    EquivalentTo: 
        (hasRated some Movie)
         and (hasRated max 1 Rating)
    
    
Class: Reviewer

    Annotations: 
        rdfs:comment "A person who reviews a movie",
        rdfs:label "Reviewer",
        <http://www.w3.org/2004/02/skos/core#broader> <http://www.ime.usp.br/~renata/FOAF-modifiedPerson>
    
    EquivalentTo: 
        Person
         and (isReviewerOf some Movie)
    
    SubClassOf: 
        Person
    
    
Class: ShortFilm

    Annotations: 
        rdfs:comment "Movie from target ontology is broader than ShortFilm as ShortFilm is a Movie but also has to have a runtime less than 40 minutes",
        rdfs:label <http://www.semanticweb.org/singh/ontologies/2020/2/CW2#ShortFilm>,
        <http://www.w3.org/2004/02/skos/core#broader> <http://www.movieontology.org/2009/11/09/Movie>
    
    EquivalentTo: 
        Movie
         and (runtime some xsd:int[< "40"^^xsd:int])
    
    SubClassOf: 
        Movie
    
    DisjointWith: 
        FeatureLengthFilm
    
    
Class: User

    SubClassOf: 
        Person
    
    
Class: Writer

    Annotations: 
        rdfs:comment "A person who writes the screenplay or script of a movie",
        rdfs:label "Writer",
        owl:sameAs <http://dbpedia.org/ontology/Writer>,
        <http://www.w3.org/2004/02/skos/core#broader> <http://www.ime.usp.br/~renata/FOAF-modifiedPerson>
    
    EquivalentTo: 
        Person
         and (isWriterOf some Movie)
    
    SubClassOf: 
        Person
    
    
Individual: <http://www.semanticweb.org/singh/ontologies/2020/2/CW2#1.0>

    Types: 
        Rating
    
    
Individual: <http://www.semanticweb.org/singh/ontologies/2020/2/CW2#2.0>

    Types: 
        Rating
    
    
Individual: <http://www.semanticweb.org/singh/ontologies/2020/2/CW2#3.0>

    Types: 
        Rating
    
    
Individual: <http://www.semanticweb.org/singh/ontologies/2020/2/CW2#4.0>

    Types: 
        Rating
    
    
Individual: <http://www.semanticweb.org/singh/ontologies/2020/2/CW2#5.0>

    Types: 
        Rating
    
    
Individual: Action

    Annotations: 
        rdfs:comment "Genre where the protagonnist protagonists are thrust into a series of events that typically include violence, fighting, frantic chasing.",
        owl:sameAs <http://www.movieontology.org/2009/10/01/movieontology.owl#Action>
    
    Types: 
        Genre
    
    
Individual: Adventure

    Annotations: 
        rdfs:comment "uses action scenes to display and explore exotic locations in an energetic way",
        owl:sameAs <http://www.semanticweb.org/singh/ontologies/2020/2/CW2#Adventure>
    
    Types: 
        Genre
    
    
Individual: Animation

    Annotations: 
        rdfs:comment "uses computer-created images with motion for the visualization.",
        owl:sameAs <http://www.movieontology.org/2009/10/01/movieontology.owl#Animation>
    
    Types: 
        Genre
    
    
Individual: Children

    Annotations: 
        rdfs:comment "movies specifically created for kids and children",
        owl:sameAs <http://www.movieontology.org/2009/10/01/movieontology.owl#Family>
    
    Types: 
        Genre
    
    
Individual: Comedy

    Annotations: 
        rdfs:comment "main emphasis is on humor",
        owl:sameAs <http://www.movieontology.org/2009/10/01/movieontology.owl#Comedy>
    
    Types: 
        Genre
    
    
Individual: Crime

    Annotations: 
        rdfs:comment "plot concernes about aspects of the crime and its detection",
        owl:sameAs <http://www.movieontology.org/2009/10/01/movieontology.owl#Crime>
    
    Types: 
        Genre
    
    
Individual: Desperado

    Types: 
        Movie
    
    Facts:  
     hasGenre  Western
    
    
Individual: Documentary

    Annotations: 
        rdfs:comment "plot is a non-fictional and intended to document the reality",
        owl:sameAs <http://www.movieontology.org/2009/10/01/movieontology.owl#Biography>,
        owl:sameAs <http://www.movieontology.org/2009/10/01/movieontology.owl#Documentary>
    
    Types: 
        Genre
    
    
Individual: Drama

    Annotations: 
        rdfs:comment "plot intended to be more serious than humorous in tone.",
        owl:sameAs <http://www.movieontology.org/2009/10/01/movieontology.owl#Drama>
    
    Types: 
        Genre
    
    
Individual: Fantasy

    Annotations: 
        rdfs:comment "plot uses fantastic themes asmagic, mythologyor exotic fantasy worlds",
        owl:sameAs <http://www.movieontology.org/2009/10/01/movieontology.owl#Fantasy>
    
    Types: 
        Genre
    
    
Individual: Film-Noir

    Annotations: 
        rdfs:comment "stylish Hollywood crime dramas, particularly those that emphasize cynical attitudes and sexual motivations",
        owl:sameAs <http://www.movieontology.org/2009/10/01/movieontology.owl#Film-Noir>
    
    Types: 
        Genre
    
    
Individual: Horror

    Annotations: 
        rdfs:comment "seeks to elicit fear for entertainment purposes.",
        owl:sameAs <http://www.movieontology.org/2009/10/01/movieontology.owl#Horror>
    
    Types: 
        Genre
    
    
Individual: IMAX

    Annotations: 
        rdfs:comment "genre that specifies the movies used high-resolution cameras, film formats, film projectors an are screened in theaters known for having very large screens"
    
    Types: 
        Genre
    
    
Individual: JohnLasseter

    Types: 
        Person
    
    Facts:  
     isDirectorOf  ToyStory,
     isWriterOf  ToyStory
    
    
Individual: Musical

    Annotations: 
        rdfs:comment "genre in which characters in the movie sing and or dance which interwove into the narrative of the movie.",
        owl:sameAs <http://www.movieontology.org/2009/10/01/movieontology.owl#Music>,
        owl:sameAs <http://www.movieontology.org/2009/10/01/movieontology.owl#Musical>
    
    Types: 
        Genre
    
    
Individual: Mystery

    Annotations: 
        rdfs:comment "movie genre that revolves around the solution of a problem or a crime. Generally a private investigator, amateur sleuth tries to solve th case by looking for clues, make dedcutions and investigation.",
        owl:sameAs <http://www.movieontology.org/2009/10/01/movieontology.owl#Mystery>
    
    Types: 
        Genre
    
    
Individual: Romance

    Annotations: 
        rdfs:comment "film genre in which the plo often focus on a romantic love storie between the main characters.",
        owl:sameAs <http://www.movieontology.org/2009/10/01/movieontology.owl#Romance>
    
    Types: 
        Genre
    
    
Individual: Sci-Fi

    Annotations: 
        rdfs:comment "genre of speculative fiction that often the plot concernes about futuristic concepts such as advanced science and technology, space exploration, time travel, parallel universes and extraterrestrial life.",
        owl:sameAs <http://www.movieontology.org/2009/10/01/movieontology.owl#Sci-Fi>
    
    Types: 
        Genre
    
    
Individual: Thriller

    Annotations: 
        rdfs:comment "also known as suspense film or suspense thriller, is a broad film genre that evokes excitement and suspense in the audience",
        owl:sameAs <http://www.movieontology.org/2009/10/01/movieontology.owl#Thriller>
    
    Types: 
        Genre
    
    
Individual: ToyStory

    Types: 
        Movie
    
    Facts:  
     hasGenre  Adventure,
     hasGenre  Animation,
     hasGenre  Children,
     hasGenre  Comedy,
     hasGenre  Fantasy,
     releaseYear  "1995"^^xsd:int,
     runtime  "127"^^xsd:int
    
    
Individual: War

    Annotations: 
        rdfs:comment "film genre about warfare, tgenerally concerned about naval, air or land battels with combat scenes central to the drama.",
        owl:sameAs <http://www.movieontology.org/2009/10/01/movieontology.owl#War>
    
    Types: 
        Genre
    
    
Individual: Western

    Annotations: 
        rdfs:comment "film genre where stories set in the atter half of the 19th century in the American Old West, generally centering the plot on the life of a cowboy or gunfighter armed with a revolver and a rifle who rides a horse.",
        owl:sameAs <http://www.movieontology.org/2009/10/01/movieontology.owl#Western>
    
    Types: 
        Genre
    
    
